lifter: deal with add with carry
during testing it turned out that add with carry (adc) and sub with
carry (sbc) could not be lifted. This is fixed now. This required some
more general handling of NZCV expressions, since the carry was fixed
before.

src/tools/lifter/bir_inst_liftingLib.sml
@@ -136,6 +136,7 @@ functor bir_inst_liftingFunctor (MD : sig val mr : bmr_rec end) : bir_inst_lifti
   val hex_code = "B4000040"
   val hex_code = "54000089"
   val hex_code = "90000000"
+  val hex_code = "DA020000";
 
   (* M0 *)
   val hex_code = "3202"
@@ -829,7 +830,8 @@ functor bir_inst_liftingFunctor (MD : sig val mr : bmr_rec end) : bir_inst_lifti
          bir_temp_varsTheory.bir_temp_var_name_def,
          bir_bool_expTheory.bir_exp_true_def,
          bir_bool_expTheory.bir_exp_false_def,
-         bir_nzcv_expTheory.BExp_nzcv_ADD_vars_of, bir_nzcv_expTheory.BExp_nzcv_SUB_vars_of]
+         bir_nzcv_expTheory.BExp_nzcv_ADD_vars_of, bir_nzcv_expTheory.BExp_nzcv_SUB_vars_of,
+         bir_nzcv_expTheory.BExp_ADD_WITH_CARRY_vars_of]
 
      val comp_upd_imm_varname_conv = SIMP_CONV (list_ss++stringSimps.STRING_ss) [bir_temp_varsTheory.bir_temp_var_def, bir_envTheory.bir_var_name_def, bir_temp_varsTheory.bir_temp_var_name_def]
 
