src/core-props/bir_nzcv_expScript.sml
@@ -33,7 +33,15 @@ val _ = new_theory "bir_nzcv_exp";
 (* Constants *)
 (*************)
 
-(* Let's instroduce constants for the components of the nzcv tuple. *)
+(* General constants for add with carry *)
+val awc_BIR_C_def = Define `awc_BIR_C w1 w2 c = FST (SND (add_with_carry (w1, w2, c)))`
+val awc_BIR_V_def = Define `awc_BIR_V w1 w2 c = SND (SND (add_with_carry (w1, w2, c)))`
+val awc_BIR_N_def = Define `awc_BIR_N w1 w2 c = (w1 + w2 + (if c then 1w else 0w) < 0w)`;
+val awc_BIR_Z_def = Define `awc_BIR_Z w1 w2 c = (w1 + w2 + (if c then 1w else 0w) = 0w)`
+
+
+(* Let's instroduce constants for the components of the nzcv tuple. Later we show that
+   these correspond to simple subtraction. *)
 val nzcv_BIR_SUB_N_def = Define `nzcv_BIR_SUB_N w1 w2 = (let (n, z, c, v) = nzcv w1 w2 in n)`;
 val nzcv_BIR_SUB_Z_def = Define `nzcv_BIR_SUB_Z w1 w2 = (let (n, z, c, v) = nzcv w1 w2 in z)`;
 val nzcv_BIR_SUB_C_def = Define `nzcv_BIR_SUB_C w1 w2 = (let (n, z, c, v) = nzcv w1 w2 in c)`;
@@ -61,30 +69,74 @@ val nzcv_BIR_ADD_Z_def = Define `nzcv_BIR_ADD_Z (w1 : 'a word) (w2 : 'a word) <=
 val nzcv_BIR_ADD_N_def = Define `nzcv_BIR_ADD_N (w1 : 'a word) (w2 : 'a word) <=>
    nzcv_BIR_SUB_N w1 (-w2)`;
 
+
 (******************)
 (* add_with_carry *)
 (******************)
 
+val nzcv_BIR_SUB_N_CARRY_DEF = store_thm ("nzcv_BIR_SUB_N_CARRY_DEF",
+  ``!w1 w2. nzcv_BIR_SUB_N w1 w2 = awc_BIR_N w1 (~w2) T``,
+SIMP_TAC std_ss [awc_BIR_N_def, ADD_WITH_CARRY_SUB, nzcv_BIR_SUB_N_def,
+  nzcv_def, LET_THM, word_msb_neg,
+  GSYM word_add_n2w, n2w_w2n] >>
+SIMP_TAC (std_ss++wordsLib.WORD_ss) [wordsTheory.WORD_NEG]);
+
+val nzcv_BIR_SUB_Z_CARRY_DEF = store_thm ("nzcv_BIR_SUB_Z_CARRY_DEF",
+  ``!w1 w2. nzcv_BIR_SUB_Z w1 w2 = awc_BIR_Z w1 (~w2) T``,
+SIMP_TAC std_ss [awc_BIR_Z_def, ADD_WITH_CARRY_SUB, nzcv_BIR_SUB_Z_def,
+  nzcv_def, LET_THM, GSYM word_add_n2w, n2w_w2n] >>
+SIMP_TAC (std_ss++wordsLib.WORD_ss) [wordsTheory.WORD_NEG]);
+
 val nzcv_BIR_SUB_C_CARRY_DEF = store_thm ("nzcv_BIR_SUB_C_CARRY_DEF",
-  ``!w1 w2. nzcv_BIR_SUB_C w1 w2 = FST (SND (add_with_carry (w1, ~w2, T)))``,
+  ``!w1 w2. nzcv_BIR_SUB_C w1 w2 = awc_BIR_C w1 (~w2) T``,
 SIMP_TAC std_ss [ADD_WITH_CARRY_SUB, nzcv_BIR_SUB_C_def, GSYM word_hs_def,
-  WORD_HIGHER_EQ]);
+  WORD_HIGHER_EQ, awc_BIR_C_def]);
 
 val nzcv_BIR_SUB_V_CARRY_DEF = store_thm ("nzcv_BIR_SUB_V_CARRY_DEF",
-  ``!w1 w2. nzcv_BIR_SUB_V w1 w2 = SND (SND (add_with_carry (w1, ~w2, T)))``,
+  ``!w1 w2. nzcv_BIR_SUB_V w1 w2 = awc_BIR_V w1 (~w2) T``,
 SIMP_TAC std_ss [ADD_WITH_CARRY_SUB, nzcv_BIR_SUB_V_def, nzcv_def, LET_THM,
-  GSYM word_add_def, word_sub_def]);
+  GSYM word_add_def, word_sub_def, awc_BIR_V_def]);
+
+
+val nzcv_BIR_ADD_N_CARRY_DEF = store_thm ("nzcv_BIR_ADD_N_CARRY_DEF",
+  ``!w1 w2. nzcv_BIR_ADD_N w1 w2 = awc_BIR_N w1 w2 F``,
+SIMP_TAC (std_ss++wordsLib.WORD_ss) [awc_BIR_N_def, ADD_WITH_CARRY_SUB, nzcv_BIR_ADD_N_def,
+  nzcv_BIR_SUB_N_def, nzcv_def, LET_THM, word_msb_neg, GSYM word_add_n2w,
+  n2w_w2n]);
+
+val nzcv_BIR_ADD_Z_CARRY_DEF = store_thm ("nzcv_BIR_ADD_Z_CARRY_DEF",
+  ``!w1 w2. nzcv_BIR_ADD_Z w1 w2 = awc_BIR_Z w1 w2 F``,
+SIMP_TAC (std_ss++wordsLib.WORD_ss) [awc_BIR_Z_def, ADD_WITH_CARRY_SUB,
+  nzcv_BIR_ADD_Z_def, nzcv_BIR_SUB_Z_def,
+  nzcv_def, LET_THM, GSYM word_add_n2w, n2w_w2n]);
 
 val nzcv_BIR_ADD_C_CARRY_DEF = store_thm ("nzcv_BIR_ADD_C_CARRY_DEF",
-  ``!w1 w2. nzcv_BIR_ADD_C w1 w2 = FST (SND (add_with_carry (w1, w2, F)))``,
+  ``!w1 w2. nzcv_BIR_ADD_C w1 w2 = awc_BIR_C w1 w2 F``,
 SIMP_TAC arith_ss [nzcv_BIR_ADD_C_def, add_with_carry_def, LET_THM,
-   bir_auxiliaryTheory.BIT_ADD_WORD_CARRY, w2n_n2w, ZERO_LT_dimword]);
+   bir_auxiliaryTheory.BIT_ADD_WORD_CARRY, w2n_n2w, ZERO_LT_dimword,
+   awc_BIR_C_def]);
 
 val nzcv_BIR_ADD_V_CARRY_DEF = store_thm ("nzcv_BIR_ADD_V_CARRY_DEF",
-  ``!w1 w2. nzcv_BIR_ADD_V w1 w2 = SND (SND (add_with_carry (w1, w2, F)))``,
+  ``!w1 w2. nzcv_BIR_ADD_V w1 w2 = awc_BIR_V w1 w2 F``,
 SIMP_TAC std_ss [add_with_carry_def, nzcv_BIR_ADD_V_def, LET_THM,
-  GSYM word_add_def] >>
+  GSYM word_add_def, awc_BIR_V_def] >>
 METIS_TAC[]);
+
+
+val awc_BIR_NZVC_INTROS = save_thm ("awc_BIR_NZVC_INTROS",
+LIST_CONJ [
+  nzcv_BIR_SUB_N_CARRY_DEF,
+  nzcv_BIR_SUB_Z_CARRY_DEF,
+  nzcv_BIR_SUB_V_CARRY_DEF,
+  nzcv_BIR_SUB_C_CARRY_DEF,
+  nzcv_BIR_ADD_N_CARRY_DEF,
+  nzcv_BIR_ADD_Z_CARRY_DEF,
+  nzcv_BIR_ADD_V_CARRY_DEF,
+  nzcv_BIR_ADD_C_CARRY_DEF]);
+
+val awc_BIR_NZVC_ELIMS = save_thm ("awc_BIR_NZVC_ELIMS",
+GSYM awc_BIR_NZVC_INTROS);
+
 
 
 (***********************)
@@ -130,12 +182,23 @@ MATCH_MP_TAC bitTheory.NOT_BIT_GT_TWOEXP >>
 SIMP_TAC std_ss [GSYM dimword_def, w2n_lt]);
 
 
-val nzcv_BIR_SUB_C_raw_aux = prove (``!w1 w2. ((w1 >=+ -w2) /\ (w2 <> 0w)) <=> (w1 >+ ~w2)``,
+val nzcv_BIR_ADD_C_raw_aux = prove (``!w1 w2. ((w1 >=+ -w2) /\ (w2 <> 0w)) <=> (w1 >+ ~w2)``,
 REPEAT Cases >>
 ASM_SIMP_TAC arith_ss [WORD_HS, w2n_n2w, word_2comp_n2w, n2w_11,
   ZERO_LT_dimword] >>
 ASM_SIMP_TAC (arith_ss++boolSimps.CONJ_ss) [] >>
 ASM_SIMP_TAC arith_ss [word_1comp_n2w, w2n_n2w, word_hi_n2w]);
+
+
+val awc_BIR_C_raw = prove (
+  ``!w1 w2 c. awc_BIR_C w1 w2 c = (if c then w1 >=+ ~w2 else (w1 >+ ~w2))``,
+
+REPEAT GEN_TAC >>
+Tactical.REVERSE (Cases_on `c`) >> SIMP_TAC std_ss [awc_BIR_NZVC_ELIMS] >- (
+  SIMP_TAC std_ss [nzcv_BIR_ADD_C_raw, nzcv_BIR_ADD_C_raw_aux]
+) >>
+Q.SUBGOAL_THEN `w2 = ~(~w2)` SUBST1_TAC >- REWRITE_TAC[WORD_NOT_NOT] >>
+SIMP_TAC std_ss [awc_BIR_NZVC_ELIMS, nzcv_BIR_SUB_C_raw, WORD_NOT_NOT]);
 
 
 val nzcv_BIR_SUB_V_raw = prove (
@@ -178,9 +241,22 @@ val nzcv_BIR_ADD_NZCV_REWRS = store_thm ("nzcv_BIR_ADD_NZCV_REWRS", ``
 
 SIMP_TAC std_ss [nzcv_BIR_SUB_NZCV_REWRS, nzcv_BIR_ADD_N_def,
   nzcv_BIR_ADD_Z_def, word_sub_def, WORD_NEG_NEG,
-  nzcv_BIR_ADD_C_raw, nzcv_BIR_SUB_C_raw_aux,
+  nzcv_BIR_ADD_C_raw, nzcv_BIR_ADD_C_raw_aux,
   nzcv_BIR_ADD_V_raw, WORD_HIGHER
 ]);
+
+
+
+val awc_BIR_NZCV_REWRS = store_thm ("awc_BIR_NZCV_REWRS", ``
+  (!w1 (w2:'a word) c. awc_BIR_N w1 w2 c <=> w1 + w2 + (if c then 1w else 0w) < 0w) /\
+  (!w1 (w2:'a word) c. awc_BIR_Z w1 w2 c <=> (w1 + w2 + (if c then 1w else 0w) = 0w)) /\
+  (!w1 (w2:'a word) c. awc_BIR_C w1 w2 c <=> (if c then ~w2 <=+ w1 else (~w2 <+ w1))) /\
+  (!w1 (w2:'a word) c. awc_BIR_V w1 w2 c <=> ((w1 < 0w <=> w2 < 0w) /\ (w1 + w2 + (if c then 1w else 0w) < 0w <=/=> w1 < 0w)))``,
+
+SIMP_TAC (std_ss++boolSimps.LIFT_COND_ss++boolSimps.EQUIV_EXTRACT_ss) [
+  awc_BIR_N_def, awc_BIR_Z_def,
+  awc_BIR_C_raw, awc_BIR_V_def, add_with_carry_def, LET_THM,
+  word_msb_neg, GSYM word_add_n2w, n2w_w2n, WORD_HIGHER, WORD_HIGHER_EQ]);
 
 
 val nzcv_BIR_ADD_SYM = store_thm ("nzcv_BIR_ADD_SYM", ``
@@ -194,6 +270,31 @@ SIMP_TAC std_ss [nzcv_BIR_ADD_N_def, nzcv_def, LET_THM,
   nzcv_BIR_SUB_Z_def, WORD_NEG_NEG, nzcv_BIR_ADD_V_def,
   GSYM word_add_def] >>
 METIS_TAC[wordsTheory.WORD_ADD_COMM, arithmeticTheory.ADD_COMM]);
+
+
+val nzcv_BIR_ADD_SYM = store_thm ("nzcv_BIR_ADD_SYM", ``
+  (!w1 (w2:'a word). nzcv_BIR_ADD_N w1 w2 <=> nzcv_BIR_ADD_N w2 w1) /\
+  (!w1 (w2:'a word). nzcv_BIR_ADD_Z w1 w2 <=> nzcv_BIR_ADD_Z w2 w1) /\
+  (!w1 (w2:'a word). nzcv_BIR_ADD_C w1 w2 <=> nzcv_BIR_ADD_C w2 w1) /\
+  (!w1 (w2:'a word). nzcv_BIR_ADD_V w1 w2 <=> nzcv_BIR_ADD_V w2 w1)``,
+
+SIMP_TAC std_ss [nzcv_BIR_ADD_N_def, nzcv_def, LET_THM,
+  nzcv_BIR_ADD_Z_def, nzcv_BIR_SUB_N_def, nzcv_BIR_ADD_C_def,
+  nzcv_BIR_SUB_Z_def, WORD_NEG_NEG, nzcv_BIR_ADD_V_def,
+  GSYM word_add_def] >>
+METIS_TAC[wordsTheory.WORD_ADD_COMM, arithmeticTheory.ADD_COMM]);
+
+
+val awc_BIR_NZCV_SYM = store_thm ("awc_BIR_NZCV_SYM", ``
+  (!w1 (w2:'a word) c. awc_BIR_N w1 w2 c <=> awc_BIR_N w2 w1 c) /\
+  (!w1 (w2:'a word) c. awc_BIR_Z w1 w2 c <=> awc_BIR_Z w2 w1 c) /\
+  (!w1 (w2:'a word) c. awc_BIR_C w1 w2 c <=> awc_BIR_C w2 w1 c) /\
+  (!w1 (w2:'a word) c. awc_BIR_V w1 w2 c <=> awc_BIR_V w2 w1 c)``,
+
+SIMP_TAC (arith_ss++wordsLib.WORD_ss) [awc_BIR_N_def, awc_BIR_Z_def, awc_BIR_C_def,
+  add_with_carry_def, LET_THM, GSYM word_add_n2w, n2w_w2n, awc_BIR_V_def] >>
+METIS_TAC[]);
+
 
 
 (*******************)
@@ -539,8 +640,8 @@ val BExp_nzcv_ADD_V_def = Define `BExp_nzcv_ADD_V sz e1 e2 =
               (BExp_Const (n2bs 0 sz)))
            (BExp_BinPred BIExp_SignedLessThan e2
               (BExp_Const (n2bs 0 sz))))
-        (BExp_UnaryExp BIExp_Not
-           (BExp_BinPred BIExp_Equal
+        (
+           (BExp_BinPred BIExp_NotEqual
               (BExp_BinPred BIExp_SignedLessThan
                  (BExp_BinExp BIExp_Plus e1 e2) (BExp_Const (n2bs 0 sz)))
               (BExp_BinPred BIExp_SignedLessThan e1
@@ -684,6 +785,195 @@ val BExp_nzcv_ADD_C_eval = store_thm ("BExp_nzcv_ADD_C_eval",
 
 REPEAT GEN_TAC >>
 SIMP_TAC (std_ss++holBACore_ss) [BExp_nzcv_ADD_C_def, nzcv_BIR_ADD_NZCV_REWRS] >>
+REPEAT CASE_TAC >> (
+   FULL_SIMP_TAC (std_ss++holBACore_ss) []
+));
+
+
+
+(******************************)
+(* Expressions ADD WITH CARRY *)
+(******************************)
+
+(* We can now define expressions for the nzcv flags *)
+val BExp_ADD_WITH_CARRY_N_def = Define `BExp_ADD_WITH_CARRY_N sz e1 e2 ec =
+   BExp_BinPred BIExp_SignedLessThan (BExp_BinExp BIExp_Plus e1
+        (BExp_BinExp BIExp_Plus e2 (BExp_IfThenElse ec (BExp_Const (n2bs 1 sz)) (BExp_Const (n2bs 0 sz)))))
+        (BExp_Const (n2bs 0 sz))`;
+
+val BExp_ADD_WITH_CARRY_Z_def = Define `BExp_ADD_WITH_CARRY_Z sz e1 e2 ec =
+   BExp_BinPred BIExp_Equal (BExp_BinExp BIExp_Plus e1
+        (BExp_BinExp BIExp_Plus e2 (BExp_IfThenElse ec (BExp_Const (n2bs 1 sz)) (BExp_Const (n2bs 0 sz)))))
+        (BExp_Const (n2bs 0 sz))`;
+
+
+val BExp_ADD_WITH_CARRY_C_def = Define `BExp_ADD_WITH_CARRY_C e1 e2 ec =
+   BExp_IfThenElse ec
+     (BExp_BinPred BIExp_LessOrEqual (BExp_UnaryExp BIExp_Not e2) e1)
+     (BExp_BinPred BIExp_LessThan (BExp_UnaryExp BIExp_Not e2) e1)`;
+
+
+val BExp_ADD_WITH_CARRY_V_def = Define `BExp_ADD_WITH_CARRY_V sz e1 e2 ec =
+     (BExp_BinExp BIExp_And
+        (BExp_BinPred BIExp_Equal
+           (BExp_BinPred BIExp_SignedLessThan e1
+              (BExp_Const (n2bs 0 sz)))
+           (BExp_BinPred BIExp_SignedLessThan e2
+              (BExp_Const (n2bs 0 sz))))
+        (BExp_BinPred BIExp_NotEqual
+              (BExp_BinPred BIExp_SignedLessThan
+                 (BExp_BinExp BIExp_Plus e1
+                    (BExp_BinExp BIExp_Plus e2 (BExp_IfThenElse ec (BExp_Const (n2bs 1 sz)) (BExp_Const (n2bs 0 sz)))))
+                  (BExp_Const (n2bs 0 sz)))
+              (BExp_BinPred BIExp_SignedLessThan e1
+                 (BExp_Const (n2bs 0 sz)))))`;
+
+
+val BExp_ADD_WITH_CARRY_DEFS = save_thm ("BExp_ADD_WITH_CARRY_DEFS",
+  LIST_CONJ [BExp_ADD_WITH_CARRY_N_def,
+             BExp_ADD_WITH_CARRY_Z_def,
+             BExp_ADD_WITH_CARRY_C_def,
+             BExp_ADD_WITH_CARRY_V_def]);
+
+
+val BExp_ADD_WITH_CARRY_type_of = store_thm ("BExp_ADD_WITH_CARRY_type_of",``
+(!sz e1 e2 ec. (type_of_bir_exp (BExp_ADD_WITH_CARRY_N sz e1 e2 ec) = (if
+    (type_of_bir_exp ec = SOME BType_Bool) /\
+    (type_of_bir_exp e1 = SOME (BType_Imm sz)) /\
+    (type_of_bir_exp e2 = SOME (BType_Imm sz)) then SOME BType_Bool else NONE))) /\
+
+(!sz e1 e2 ec. (type_of_bir_exp (BExp_ADD_WITH_CARRY_V sz e1 e2 ec) = if
+    (type_of_bir_exp ec = SOME BType_Bool) /\
+    (type_of_bir_exp e1 = SOME (BType_Imm sz)) /\
+    (type_of_bir_exp e2 = SOME (BType_Imm sz)) then SOME BType_Bool else NONE)) /\
+
+(!e1 e2 ec sz.
+    (type_of_bir_exp (BExp_ADD_WITH_CARRY_Z sz e1 e2 ec) = if
+    (type_of_bir_exp ec = SOME BType_Bool) /\
+    (type_of_bir_exp e1 = SOME (BType_Imm sz)) /\
+    (type_of_bir_exp e2 = SOME (BType_Imm sz)) then SOME BType_Bool else NONE)) /\
+
+(!e1 e2 ec. (type_of_bir_exp (BExp_ADD_WITH_CARRY_C e1 e2 ec) = if
+    ?sz. (type_of_bir_exp ec = SOME BType_Bool) /\
+         (type_of_bir_exp e1 = SOME (BType_Imm sz)) /\
+         (type_of_bir_exp e2 = SOME (BType_Imm sz)) then SOME BType_Bool else NONE))``,
+
+SIMP_TAC (std_ss++holBACore_ss) [BExp_ADD_WITH_CARRY_DEFS, type_of_bir_exp_def,
+  pairTheory.pair_case_thm] >>
+REPEAT STRIP_TAC >> REPEAT CASE_TAC >> (
+  FULL_SIMP_TAC (std_ss++holBACore_ss) [bir_type_checker_DEFS, BType_Bool_def] >>
+  FULL_SIMP_TAC (std_ss++holBACore_ss) []
+));
+
+
+val BExp_ADD_WITH_CARRY_vars_of = store_thm ("BExp_ADD_WITH_CARRY_vars_of",``
+(!sz e1 e2 ec. (bir_vars_of_exp (BExp_ADD_WITH_CARRY_N sz e1 e2 ec) = (
+    bir_vars_of_exp e1 UNION bir_vars_of_exp e2 UNION bir_vars_of_exp ec))) /\
+
+(!sz e1 e2 ec. (bir_vars_of_exp (BExp_ADD_WITH_CARRY_V sz e1 e2 ec) = (
+    bir_vars_of_exp e1 UNION bir_vars_of_exp e2 UNION bir_vars_of_exp ec))) /\
+
+(!sz e1 e2 ec. (bir_vars_of_exp (BExp_ADD_WITH_CARRY_Z sz e1 e2 ec) = (
+    bir_vars_of_exp e1 UNION bir_vars_of_exp e2 UNION bir_vars_of_exp ec))) /\
+
+(!e1 e2 ec. (bir_vars_of_exp (BExp_ADD_WITH_CARRY_C e1 e2 ec) = (
+    bir_vars_of_exp e1 UNION bir_vars_of_exp e2 UNION bir_vars_of_exp ec)))``,
+
+SIMP_TAC (std_ss++holBACore_ss++boolSimps.EQUIV_EXTRACT_ss) [BExp_ADD_WITH_CARRY_DEFS,
+  EXTENSION, IN_UNION, NOT_IN_EMPTY]);
+
+
+
+val BExp_ADD_WITH_CARRY_N_eval = store_thm ("BExp_ADD_WITH_CARRY_N_eval",
+``!sz e1 e2 ec env.
+  (bir_eval_exp (BExp_ADD_WITH_CARRY_N sz e1 e2 ec) env =
+     case (sz, bir_eval_exp e1 env, bir_eval_exp e2 env, bir_dest_bool_val (bir_eval_exp ec env)) of
+         (Bit1, BVal_Imm (Imm1 w1), BVal_Imm (Imm1 w2), SOME c) =>
+            BVal_Imm (bool2b (awc_BIR_N w1 w2 c))
+       | (Bit8, BVal_Imm (Imm8 w1), BVal_Imm (Imm8 w2), SOME c) =>
+            BVal_Imm (bool2b (awc_BIR_N w1 w2 c))
+       | (Bit16, BVal_Imm (Imm16 w1), BVal_Imm (Imm16 w2), SOME c) =>
+            BVal_Imm (bool2b (awc_BIR_N w1 w2 c))
+       | (Bit32, BVal_Imm (Imm32 w1), BVal_Imm (Imm32 w2), SOME c) =>
+            BVal_Imm (bool2b (awc_BIR_N w1 w2 c))
+       | (Bit64, BVal_Imm (Imm64 w1), BVal_Imm (Imm64 w2), SOME c) =>
+            BVal_Imm (bool2b (awc_BIR_N w1 w2 c))
+       | _ => BVal_Unknown)``,
+
+REPEAT GEN_TAC >>
+SIMP_TAC (std_ss++holBACore_ss) [BExp_ADD_WITH_CARRY_N_def, awc_BIR_NZCV_REWRS] >>
+REPEAT CASE_TAC >> (
+   FULL_SIMP_TAC (std_ss++holBACore_ss++wordsLib.WORD_ss++boolSimps.LIFT_COND_ss) []
+));
+
+
+val BExp_ADD_WITH_CARRY_V_eval = store_thm ("BExp_ADD_WITH_CARRY_V_eval",
+``!sz e1 e2 ec env.
+  (bir_eval_exp (BExp_ADD_WITH_CARRY_V sz e1 e2 ec) env =
+     case (sz, bir_eval_exp e1 env, bir_eval_exp e2 env, bir_dest_bool_val (bir_eval_exp ec env)) of
+         (Bit1, BVal_Imm (Imm1 w1), BVal_Imm (Imm1 w2), SOME c) =>
+            BVal_Imm (bool2b (awc_BIR_V w1 w2 c))
+       | (Bit8, BVal_Imm (Imm8 w1), BVal_Imm (Imm8 w2), SOME c) =>
+            BVal_Imm (bool2b (awc_BIR_V w1 w2 c))
+       | (Bit16, BVal_Imm (Imm16 w1), BVal_Imm (Imm16 w2), SOME c) =>
+            BVal_Imm (bool2b (awc_BIR_V w1 w2 c))
+       | (Bit32, BVal_Imm (Imm32 w1), BVal_Imm (Imm32 w2), SOME c) =>
+            BVal_Imm (bool2b (awc_BIR_V w1 w2 c))
+       | (Bit64, BVal_Imm (Imm64 w1), BVal_Imm (Imm64 w2), SOME c) =>
+            BVal_Imm (bool2b (awc_BIR_V w1 w2 c))
+       | _ => BVal_Unknown)``,
+
+REPEAT GEN_TAC >>
+SIMP_TAC (std_ss++holBACore_ss) [BExp_ADD_WITH_CARRY_V_def, awc_BIR_NZCV_REWRS] >>
+REPEAT CASE_TAC >> (
+   FULL_SIMP_TAC (std_ss++holBACore_ss++wordsLib.WORD_ss) [
+     bir_bin_pred_BOOL_OPER_EVAL,
+     bir_unary_exp_BOOL_OPER_EVAL,
+     bir_bin_exp_BOOL_OPER_EVAL]
+));
+
+
+val BExp_ADD_WITH_CARRY_Z_eval = store_thm ("BExp_ADD_WITH_CARRY_Z_eval",
+``!sz e1 e2 ec env.
+  (bir_eval_exp (BExp_ADD_WITH_CARRY_Z sz e1 e2 ec) env =
+     case (sz, bir_eval_exp e1 env, bir_eval_exp e2 env, bir_dest_bool_val (bir_eval_exp ec env)) of
+         (Bit1, BVal_Imm (Imm1 w1), BVal_Imm (Imm1 w2), SOME c) =>
+            BVal_Imm (bool2b (awc_BIR_Z w1 w2 c))
+       | (Bit8, BVal_Imm (Imm8 w1), BVal_Imm (Imm8 w2), SOME c) =>
+            BVal_Imm (bool2b (awc_BIR_Z w1 w2 c))
+       | (Bit16, BVal_Imm (Imm16 w1), BVal_Imm (Imm16 w2), SOME c) =>
+            BVal_Imm (bool2b (awc_BIR_Z w1 w2 c))
+       | (Bit32, BVal_Imm (Imm32 w1), BVal_Imm (Imm32 w2), SOME c) =>
+            BVal_Imm (bool2b (awc_BIR_Z w1 w2 c))
+       | (Bit64, BVal_Imm (Imm64 w1), BVal_Imm (Imm64 w2), SOME c) =>
+            BVal_Imm (bool2b (awc_BIR_Z w1 w2 c))
+       | _ => BVal_Unknown)``,
+
+REPEAT GEN_TAC >>
+SIMP_TAC (std_ss++holBACore_ss) [BExp_ADD_WITH_CARRY_Z_def, awc_BIR_NZCV_REWRS] >>
+REPEAT CASE_TAC >> (
+   FULL_SIMP_TAC (std_ss++holBACore_ss++wordsLib.WORD_ss++boolSimps.LIFT_COND_ss) []
+));
+
+
+val BExp_ADD_WITH_CARRY_C_eval = store_thm ("BExp_ADD_WITH_CARRY_C_eval",
+``!e1 e2 ec env.
+  (bir_eval_exp (BExp_ADD_WITH_CARRY_C e1 e2 ec) env =
+     case (bir_eval_exp e1 env, bir_eval_exp e2 env, bir_dest_bool_val (bir_eval_exp ec env)) of
+         (BVal_Imm (Imm1 w1), BVal_Imm (Imm1 w2), SOME c) =>
+            BVal_Imm (bool2b (awc_BIR_C w1 w2 c))
+       | (BVal_Imm (Imm8 w1), BVal_Imm (Imm8 w2), SOME c) =>
+            BVal_Imm (bool2b (awc_BIR_C w1 w2 c))
+       | (BVal_Imm (Imm16 w1), BVal_Imm (Imm16 w2), SOME c) =>
+            BVal_Imm (bool2b (awc_BIR_C w1 w2 c))
+       | (BVal_Imm (Imm32 w1), BVal_Imm (Imm32 w2), SOME c) =>
+            BVal_Imm (bool2b (awc_BIR_C w1 w2 c))
+       | (BVal_Imm (Imm64 w1), BVal_Imm (Imm64 w2), SOME c) =>
+            BVal_Imm (bool2b (awc_BIR_C w1 w2 c))
+       | _ => BVal_Unknown)``,
+
+REPEAT GEN_TAC >>
+SIMP_TAC (std_ss++holBACore_ss) [BExp_ADD_WITH_CARRY_C_def, awc_BIR_NZCV_REWRS] >>
 REPEAT CASE_TAC >> (
    FULL_SIMP_TAC (std_ss++holBACore_ss) []
 ));
