src/tools/lifter/bir_nzcv_introsScript.sml
@@ -24,7 +24,7 @@ val nzcv_SUB_V_fold_ARM8 = store_thm ("nzcv_SUB_V_fold_ARM8",
   nzcv_BIR_SUB_V w0 w1``,
 
 REPEAT GEN_TAC >>
-SIMP_TAC std_ss [nzcv_BIR_SUB_V_CARRY_DEF,
+SIMP_TAC std_ss [nzcv_BIR_SUB_V_CARRY_DEF, awc_BIR_V_def,
   add_with_carry_def, LET_THM, word_msb_n2w]);
 
 
@@ -36,7 +36,7 @@ val nzcv_SUB_C_fold_ARM8 = store_thm ("nzcv_SUB_C_fold_ARM8",
 
 REPEAT GEN_TAC >>
 SIMP_TAC (std_ss++boolSimps.LIFT_COND_ss) [nzcv_BIR_SUB_C_CARRY_DEF, add_with_carry_def, LET_THM,
-   ZERO_LT_dimword, w2n_n2w]);
+   ZERO_LT_dimword, w2n_n2w, awc_BIR_C_def]);
 
 
 val nzcv_SUB_Z_fold_ARM8 = store_thm ("nzcv_SUB_Z_fold_ARM8",
@@ -66,7 +66,7 @@ val nzcv_ADD_V_fold_ARM8 = store_thm ("nzcv_ADD_V_fold_ARM8",
   (word_msb w0 <=> word_msb w1) /\
   (word_msb w0 <=/=> BIT (dimindex (:'a) - 1) (w2n w0 + w2n w1)) = nzcv_BIR_ADD_V w0 w1``,
 
-SIMP_TAC std_ss [nzcv_BIR_ADD_V_CARRY_DEF,
+SIMP_TAC std_ss [nzcv_BIR_ADD_V_CARRY_DEF, awc_BIR_V_def,
   add_with_carry_def, LET_THM, GSYM word_msb_n2w]);
 
 
@@ -86,7 +86,7 @@ val nzcv_ADD_C_fold_ARM8 = store_thm ("nzcv_ADD_C_fold_ARM8",
 
 REPEAT GEN_TAC >>
 SIMP_TAC (arith_ss++boolSimps.LIFT_COND_ss) [nzcv_BIR_ADD_C_CARRY_DEF, add_with_carry_def,
-  LET_THM, ZERO_LT_dimword, w2n_n2w]);
+  LET_THM, ZERO_LT_dimword, w2n_n2w, awc_BIR_C_def]);
 
 
 val nzcv_ADD_Z_fold_ARM8 = store_thm ("nzcv_ADD_Z_fold_ARM8",
@@ -104,6 +104,114 @@ val nzcv_ADD_FOLDS_ARM8_GEN = save_thm ("nzcv_ADD_FOLDS_ARM8_GEN",
   LIST_CONJ [nzcv_ADD_N_fold_ARM8, nzcv_ADD_C_fold_ARM8, nzcv_ADD_Z_fold_ARM8, nzcv_ADD_V_fold_ARM8,
     nzcv_ADD_V_fold_ARM8_ID]
 )
+
+
+(*************************)
+(* ARM 8 add_with_carry  *)
+(*************************)
+
+(* cmp uses w2 - w1, we also need a version for w1 + w2. *)
+
+val awc_BIR_V_fold_ARM8 = store_thm ("awc_BIR_V_fold_ARM8",
+``!w1:'a word w0:'a word c.
+  (word_msb w0 <=> word_msb w1) /\
+  (word_msb w0 <=/=> BIT (dimindex (:'a) - 1) (w2n w0 + w2n w1 + (if c then 1 else 0))) = awc_BIR_V w0 w1 c``,
+
+SIMP_TAC std_ss [awc_BIR_V_def,
+  add_with_carry_def, LET_THM, GSYM word_msb_n2w]);
+
+
+val awc_BIR_V_fold_ARM8_ID = store_thm ("awc_BIR_V_fold_ARM8_ID",
+``!w:'a word c.
+  (word_msb w <=/=> BIT (dimindex (:'a) - 1) (w2n w + w2n w + (if c then 1 else 0))) = awc_BIR_V w w c``,
+SIMP_TAC std_ss [GSYM awc_BIR_V_fold_ARM8]);
+
+
+val awc_BIR_C_fold_ARM8 = store_thm ("awc_BIR_C_fold_ARM8",
+``!w1 w0 c.
+  ((if w2n w0 + ((w2n (w1:'a word)) + if c then 1 else (0:num)) < dimword (:'a) then
+       w2n w0 + (w2n w1 + if c then 1 else 0)
+  else (w2n w0 + (w2n w1 + if c then 1 else 0)) MOD (dimword (:'a))) <>
+  w2n w0 + (w2n w1 + if c then 1 else 0)) = awc_BIR_C w0 w1 c``,
+
+REPEAT GEN_TAC >>
+SIMP_TAC (arith_ss++boolSimps.LIFT_COND_ss) [add_with_carry_def,
+  LET_THM, ZERO_LT_dimword, w2n_n2w, awc_BIR_C_def]);
+
+
+val awc_BIR_Z_fold_ARM8 = store_thm ("awc_BIR_Z_fold_ARM8",
+``!w1 (w0 : 'a word) c.
+     ((n2w (w2n w0 + ((w2n w1 + if c then 1 else 0)))) = (0w:'a word)) <=>
+     awc_BIR_Z w0 w1 c``,
+SIMP_TAC (std_ss++boolSimps.LIFT_COND_ss++wordsLib.WORD_ss) [awc_BIR_Z_def, GSYM word_add_n2w, n2w_w2n]);
+
+val awc_BIR_N_fold_ARM8 = store_thm ("awc_BIR_N_fold_ARM8",
+``!w1 w0 c. BIT (dimindex (:'a) - 1) ((w2n w0 + ((w2n w1 + if c then 1 else 0)))) =
+            awc_BIR_N (w0:'a word) w1 c``,
+SIMP_TAC std_ss [awc_BIR_N_def, GSYM word_msb_n2w, GSYM word_add_n2w,
+  n2w_w2n, word_msb_neg] >>
+SIMP_TAC (std_ss++boolSimps.LIFT_COND_ss++wordsLib.WORD_ss) []);
+
+
+val awc_BIR_RES_fold_ARM8 = store_thm ("awc_BIR_RES_fold_ARM8",
+``!w0 w1 c. (n2w (w2n w0 + ((w2n w1 + if c then 1 else 0)))) =
+            (w0 + w1 + (if c then 1w else 0w))``,
+SIMP_TAC (std_ss++boolSimps.LIFT_COND_ss++wordsLib.WORD_ss) [
+  GSYM word_add_n2w, n2w_w2n]);
+
+
+val awc_BIR_RES_FOLD_SUB = store_thm ("awc_BIR_RES_FOLD_SUB",
+``!w1:'a word w2 c.
+     (w1 + (~w2) + (if c then 1w else 0w)) =
+     (w1 - w2 - (if c then 0w else 1w))``,
+
+SIMP_TAC std_ss [WORD_NEG, word_sub_def] >>
+SIMP_TAC (std_ss++wordsLib.WORD_ss++boolSimps.LIFT_COND_ss) []);
+
+val awc_BIR_Z_nzcv_BIR_SUB_Z_fold = prove (
+  ``!(w0:'a word) w1 c. nzcv_BIR_SUB_Z (w0 - w1) (if c then 0w else 1w) =
+                        awc_BIR_Z w0 (~w1) c``,
+
+SIMP_TAC std_ss [GSYM awc_BIR_Z_fold_ARM8, GSYM nzcv_SUB_Z_fold_ARM8,
+  awc_BIR_RES_fold_ARM8, awc_BIR_RES_FOLD_SUB]);
+
+val awc_BIR_Z_nzcv_BIR_ADD_Z_fold = prove (
+  ``!(w0:'a word) w1 c. nzcv_BIR_ADD_Z (w0 + w1) (if c then 1w else 0w) =
+                        awc_BIR_Z w0 w1 c``,
+
+SIMP_TAC std_ss [GSYM awc_BIR_Z_fold_ARM8, GSYM nzcv_ADD_Z_fold_ARM8,
+  awc_BIR_RES_fold_ARM8, awc_BIR_RES_FOLD_SUB]);
+
+val awc_BIR_Z_nzcv_BIR_SUB_N_fold = prove (
+  ``!(w0:'a word) w1 c. nzcv_BIR_SUB_N (w0 - w1) (if c then 0w else 1w) =
+                        awc_BIR_N w0 (~w1) c``,
+
+SIMP_TAC std_ss [GSYM awc_BIR_N_fold_ARM8, GSYM nzcv_SUB_N_fold_ARM8,
+  awc_BIR_RES_fold_ARM8, awc_BIR_RES_FOLD_SUB, GSYM word_msb_n2w]);
+
+val awc_BIR_Z_nzcv_BIR_ADD_N_fold = prove (
+  ``!(w0:'a word) w1 c. nzcv_BIR_ADD_N (w0 + w1) (if c then 1w else 0w) =
+                        awc_BIR_N w0 w1 c``,
+
+SIMP_TAC std_ss [GSYM awc_BIR_N_fold_ARM8, GSYM nzcv_ADD_N_fold_ARM8,
+  awc_BIR_RES_fold_ARM8, awc_BIR_RES_FOLD_SUB, GSYM word_msb_n2w]);
+
+
+
+val awc_BIR_NZCV_FOLDS_ARM8_GEN = save_thm ("awc_BIR_NZCV_FOLDS_ARM8_GEN",
+  LIST_CONJ [
+    awc_BIR_N_fold_ARM8,
+    SIMP_RULE std_ss [awc_BIR_RES_fold_ARM8, GSYM arithmeticTheory.ADD_ASSOC] awc_BIR_Z_fold_ARM8,
+    awc_BIR_C_fold_ARM8,
+    SIMP_RULE std_ss [awc_BIR_N_fold_ARM8, GSYM arithmeticTheory.ADD_ASSOC] awc_BIR_V_fold_ARM8,
+    SIMP_RULE std_ss [awc_BIR_N_fold_ARM8, GSYM arithmeticTheory.ADD_ASSOC] awc_BIR_V_fold_ARM8_ID,
+    awc_BIR_RES_fold_ARM8,
+    awc_BIR_RES_FOLD_SUB,
+    awc_BIR_Z_nzcv_BIR_SUB_Z_fold,
+    awc_BIR_Z_nzcv_BIR_ADD_Z_fold,
+    awc_BIR_Z_nzcv_BIR_SUB_N_fold,
+    awc_BIR_Z_nzcv_BIR_ADD_N_fold
+  ])
 
 
 (************************)
@@ -220,15 +328,17 @@ val nzcv_FOLDS_ARM8_gen_size = LIST_CONJ [
       nzcv_SUB_FOLDS_ARM8_GEN,
       nzcv_SUB_FOLDS_ARM8_CONST_GEN,
       nzcv_ADD_FOLDS_ARM8_GEN,
-      nzcv_ADD_FOLDS_ARM8_CONST_GEN];
+      nzcv_ADD_FOLDS_ARM8_CONST_GEN,
+      awc_BIR_NZCV_FOLDS_ARM8_GEN];
 
 
 val nzcv_FOLDS_ARM8 = save_thm ("nzcv_FOLDS_ARM8",
+SIMP_RULE (std_ss) [arithmeticTheory.ADD_ASSOC] (
 SIMP_RULE (std_ss++wordsLib.SIZES_ss) []  (LIST_CONJ [
   INST_TYPE [``:'a`` |-> ``:32``] nzcv_FOLDS_ARM8_gen_size,
   INST_TYPE [``:'a`` |-> ``:64``] nzcv_FOLDS_ARM8_gen_size
  ]
-));
+)));
 
 
 
@@ -291,21 +401,23 @@ test_nzcv_folds_hex "1b000001"
 (* ARM 0 *)
 (*********)
 
-val nzcv_SUB_C_fold_M0 = store_thm ("nzcv_SUB_C_fold_M0",
-``!w1 w0. (CARRY_OUT w0 (~w1) T) = nzcv_BIR_SUB_C w0 w1``,
-REWRITE_TAC[nzcv_BIR_SUB_C_CARRY_DEF]);
+val awc_BIR_C_fold_M0 = store_thm ("awc_BIR_C_fold_M0",
+``!w1 w0 c. CARRY_OUT w0 w1 c = awc_BIR_C w0 w1 c``,
+REWRITE_TAC[awc_BIR_C_def]);
 
-val nzcv_SUB_V_fold_M0 = store_thm ("nzcv_SUB_V_fold_M0",
-``!w1 w0. (OVERFLOW w0 (~w1) T) = nzcv_BIR_SUB_V w0 w1``,
-REWRITE_TAC[nzcv_BIR_SUB_V_CARRY_DEF])
+val awc_BIR_RES_fold_M0 = store_thm ("awc_BIR_RES_fold_M0",
+``!w0 w1 c. FST (add_with_carry (w0,w1,c)) =
+            w0 + w1 + (if c then 1w else 0w)``,
+SIMP_TAC arith_ss [add_with_carry_def, LET_THM,
+  awc_BIR_RES_fold_ARM8]);
 
-val nzcv_ADD_C_fold_M0 = store_thm ("nzcv_SUB_C_fold_M0",
-``!w1 w0. (CARRY_OUT w0 w1 F) = nzcv_BIR_ADD_C w0 w1``,
-REWRITE_TAC[nzcv_BIR_ADD_C_CARRY_DEF])
+val awc_BIR_Z_fold_M0 = store_thm ("awc_BIR_Z_fold_M0",
+``!w1 w0 c. ((w0 + w1 + (if c then 1w else 0w)) = 0w) <=> awc_BIR_Z w0 w1 c``,
+REWRITE_TAC[awc_BIR_Z_def]);
 
-val nzcv_ADD_V_fold_M0 = store_thm ("nzcv_ADD_V_fold_M0",
-``!w1 w0. (OVERFLOW w0 w1 F) = nzcv_BIR_ADD_V w0 w1``,
-REWRITE_TAC[nzcv_BIR_ADD_V_CARRY_DEF])
+val awc_BIR_V_fold_M0 = store_thm ("awc_BIR_V_fold_M0",
+``!w1 w0 c. OVERFLOW w0 w1 c = awc_BIR_V w0 w1 c``,
+REWRITE_TAC[awc_BIR_V_def]);
 
 val nzcv_SUB_N_fold_M0 = store_thm ("nzcv_SUB_N_fold_M0",
 ``!w1:word32 w0. (word_bit 31 (w0 - w1)) = nzcv_BIR_SUB_N w0 w1``,
@@ -321,15 +433,22 @@ val nzcv_SUB_Z_fold_M0 = store_thm ("nzcv_SUB_Z_fold_M0",
 ``!w1 w0. (w0 - w1 = 0w) = nzcv_BIR_SUB_Z w0 w1``,
 REWRITE_TAC[nzcv_SUB_Z_fold_ARM8]);
 
-val nzcv_ADD_Z_fold_M0 = store_thm ("nzcv_SUB_Z_fold_M0",
+val nzcv_ADD_Z_fold_M0 = store_thm ("nzcv_ADD_Z_fold_M0",
 ``!w1 w0. (w0 + w1 = 0w) = nzcv_BIR_ADD_Z w0 w1``,
 REWRITE_TAC[nzcv_ADD_Z_fold_ARM8]);
 
 val nzcv_FOLDS_M0 = save_thm ("nzcv_FOLDS_M0",
- LIST_CONJ [nzcv_SUB_V_fold_M0, nzcv_SUB_C_fold_M0,
-            nzcv_ADD_V_fold_M0, nzcv_ADD_C_fold_M0,
+ LIST_CONJ [awc_BIR_V_fold_M0, awc_BIR_C_fold_M0,
+            awc_BIR_NZVC_ELIMS, awc_BIR_Z_fold_M0,
+            awc_BIR_RES_fold_M0, awc_BIR_RES_FOLD_SUB,
             nzcv_SUB_N_fold_M0, nzcv_ADD_N_fold_M0,
-            nzcv_SUB_Z_fold_M0, nzcv_ADD_Z_fold_M0]);
+            nzcv_SUB_Z_fold_M0, nzcv_ADD_Z_fold_M0,
+            awc_BIR_Z_nzcv_BIR_SUB_Z_fold,
+            awc_BIR_Z_nzcv_BIR_ADD_Z_fold,
+            awc_BIR_Z_nzcv_BIR_SUB_N_fold,
+            awc_BIR_Z_nzcv_BIR_ADD_N_fold
+]);
+
 
 (* Test
 
@@ -337,12 +456,15 @@ open m0_stepLib
 
 val ev = thumb_step_code (true, true);
 fun test_nzcv_folds s =
-  (map (SIMP_RULE std_ss [STEP_REWRS_M0]) (flatten (ev s)));
+  (map (SIMP_RULE std_ss [nzcv_FOLDS_M0]) (flatten (ev s)));
 
 test_nzcv_folds `adds r2, #0`
 test_nzcv_folds `adds r2, #1`
 test_nzcv_folds `subs r2, r2`
 test_nzcv_folds `cmp r0, #3`
+test_nzcv_folds `adcs r0, r1`
+test_nzcv_folds `sbcs r0, r1`
+test_nzcv_folds `sbcs r0, r0`
 test_nzcv_folds `cmn r0, r1`
 test_nzcv_folds `cmp r0, #0`
 
